@prefix dc: <http://purl.org/dc/elements/1.1/> .
@prefix dcat: <http://www.w3.org/ns/dcat#> .
@prefix dct: <http://purl.org/dc/terms/> .
@prefix euvoc: <http://publications.europa.eu/ontology/euvoc#> .
@prefix foaf: <http://xmlns.com/foaf/0.1/> .
@prefix org: <http://www.w3.org/ns/org#> .
@prefix owl: <http://www.w3.org/2002/07/owl#> .
@prefix pav: <http://purl.org/pav/> .
@prefix prov: <http://www.w3.org/ns/prov#> .
@prefix qb: <http://purl.org/linked-data/cube#> .
@prefix rdf: <http://www.w3.org/1999/02/22-rdf-syntax-ns#> .
@prefix rdfs: <http://www.w3.org/2000/01/rdf-schema#> .
@prefix schema: <http://schema.org/> .
@prefix sh: <http://www.w3.org/ns/shacl#> .
@prefix skos: <http://www.w3.org/2004/02/skos/core#> .
@prefix skosthes: <http://purl.org/iso25964/skos-thes#> .
@prefix skosxl: <http://www.w3.org/2008/05/skos-xl#> .
@prefix wetaxtop: <http://data.windenergy.dtu.dk/controlled-terminology/taxonomy-topics/> .
@prefix xsd: <http://www.w3.org/2001/XMLSchema#> .

<http://data.windenergy.dtu.dk/controlled-terminology/taxonomy-topics/> a skos:ConceptScheme;
  dct:creator <http://orcid.org/0000-0002-9381-9693>, <http://orcid.org/0000-0003-4124-9040>;
  dct:description "A taxonomical organization of research topics in wind energy which follows a typical lifecycle of wind farm development."@en;
  dct:title "Taxonomy of Research Topics in Wind Energy"@en;
  pav:createdOn "2020-12-01T00:00:00+01:00"@en;
  pav:lastUpdatedOn "2020-12-01T00:00:00+01:00"@en;
  pav:version "0.1"@en;
  skos:hasTopConcept wetaxtop:Economics, wetaxtop:OperationMaintenance, wetaxtop:Siting,
    wetaxtop:WindPowerPlant, wetaxtop:WindTurbine;
  skos:prefLabel "Wind Energy Taxonomy of Topics"@en .

wetaxtop:IEVref a rdf:Property;
  dct:creator <https://orcid.org/0000-0002-9381-9693>;
  rdfs:label "IEV ref"@en;
  skos:definition "A code used to identify certain concept in IEC Electropedia (http://www.electropedia.org/)"@en;
  skos:prefLabel "IEV ref"@en .

wetaxtop:Economics a skos:Concept;
  dct:contributor <https://orcid.org/0000-0002-9381-9693>;
  dct:creator <http://orcid.org/0000-0003-4124-9040>, <https://orcid.org/0000-0002-9381-9693>;
  skos:inScheme <http://data.windenergy.dtu.dk/controlled-terminology/taxonomy-topics/>;
  skos:narrower wetaxtop:BusinessModels, wetaxtop:LevelizedCostofEnergyModels, wetaxtop:MarketModels,
    wetaxtop:ProjectFinance, wetaxtop:SupportSchemes;
  skos:prefLabel "Economics"@en;
  skos:topConceptOf <http://data.windenergy.dtu.dk/controlled-terminology/taxonomy-topics/> .

wetaxtop:BusinessModels a skos:Concept;
  dct:contributor <https://orcid.org/0000-0002-9381-9693>;
  dct:creator <http://orcid.org/0000-0003-4124-9040>;
  skos:broader wetaxtop:Economics;
  skos:definition "A conceptual structure that supports the viability of wind energy projects and details how they operate to create profit."@en;
  skos:inScheme <http://data.windenergy.dtu.dk/controlled-terminology/taxonomy-topics/>;
  skos:prefLabel "Business Models"@en .

wetaxtop:LevelizedCostofEnergyModels a skos:Concept;
  dct:contributor <https://orcid.org/0000-0002-9381-9693>;
  dct:creator <http://orcid.org/0000-0003-4124-9040>;
  skos:broader wetaxtop:Economics;
  skos:definition "An expression of the production cost of each unit of electricity generated over the working life of the plant taking into account wind farm development costs, capital investment, financial costs and lifetime running costs."@en;
  skos:inScheme <http://data.windenergy.dtu.dk/controlled-terminology/taxonomy-topics/>;
  skos:prefLabel "Levelized Cost of Energy Models"@en .

wetaxtop:ProjectFinance a skos:Concept;
  dct:contributor <https://orcid.org/0000-0002-9381-9693>;
  dct:creator <http://orcid.org/0000-0003-4124-9040>;
  skos:broader wetaxtop:Economics;
  skos:inScheme <http://data.windenergy.dtu.dk/controlled-terminology/taxonomy-topics/>;
  skos:prefLabel "Project Finance"@en .

wetaxtop:MarketModels a skos:Concept;
  dct:contributor <https://orcid.org/0000-0002-9381-9693>;
  dct:creator <http://orcid.org/0000-0003-4124-9040>;
  skos:broader wetaxtop:Economics;
  skos:inScheme <http://data.windenergy.dtu.dk/controlled-terminology/taxonomy-topics/>;
  skos:prefLabel "Market Models"@en .

wetaxtop:SupportSchemes a skos:Concept;
  dct:contributor <https://orcid.org/0000-0002-9381-9693>;
  dct:creator <http://orcid.org/0000-0003-4124-9040>;
  skos:broader wetaxtop:Economics;
  skos:inScheme <http://data.windenergy.dtu.dk/controlled-terminology/taxonomy-topics/>;
  skos:prefLabel "Support Schemes"@en .

wetaxtop:OperationMaintenance a skos:Concept;
  wetaxtop:IEVref "192-06"@en;
  dct:contributor <https://orcid.org/0000-0002-9381-9693>;
  dct:creator <http://orcid.org/0000-0003-4124-9040>;
  skos:definition "Combination of all technical and management actions intended to retain an item in, or restore it to, a state in which it can perform as required."@en;
  skos:inScheme <http://data.windenergy.dtu.dk/controlled-terminology/taxonomy-topics/>;
  skos:narrower wetaxtop:Commissioning, wetaxtop:Decommissioning, wetaxtop:Forecasting,
    wetaxtop:HealthSafety, wetaxtop:Installation, wetaxtop:MaintenanceScheduling;
  skos:prefLabel "Operation & Maintenance"@en;
  skos:topConceptOf <http://data.windenergy.dtu.dk/controlled-terminology/taxonomy-topics/> .

wetaxtop:Commissioning a skos:Concept;
  wetaxtop:IEVref "821-12"@en;
  dct:contributor <https://orcid.org/0000-0002-9381-9693>;
  dct:creator <http://orcid.org/0000-0003-4124-9040>;
  skos:broader wetaxtop:OperationMaintenance;
  skos:definition "Activities undertaken to prepare a system or product prior to demonstrating that it meets its specified requirements."@en;
  skos:editorialNote "SOURCE: IEC 62278:2002, 3.50"@en;
  skos:inScheme <http://data.windenergy.dtu.dk/controlled-terminology/taxonomy-topics/>;
  skos:prefLabel "Commissioning"@en .

wetaxtop:Decommissioning a skos:Concept;
  wetaxtop:IEVref "395-08"@en;
  dct:contributor <https://orcid.org/0000-0002-9381-9693>;
  dct:creator <http://orcid.org/0000-0003-4124-9040>;
  skos:broader wetaxtop:OperationMaintenance;
  skos:definition "Administrative and technical actions taken to allow the removal of some or all of the regulatory controls from a facility"@en;
  skos:inScheme <http://data.windenergy.dtu.dk/controlled-terminology/taxonomy-topics/>;
  skos:narrower wetaxtop:EndofLifeExtension;
  skos:prefLabel "Decommissioning"@en .

wetaxtop:EndofLifeExtension a skos:Concept;
  wetaxtop:IEVref "904-01-17"@en;
  dct:contributor <https://orcid.org/0000-0002-9381-9693>;
  dct:creator <http://orcid.org/0000-0003-4124-9040>;
  skos:broader wetaxtop:Decommissioning;
  skos:definition "When the life cycle stage of a product instead of end is extended for a certain period."@en;
  skos:inScheme <http://data.windenergy.dtu.dk/controlled-terminology/taxonomy-topics/>;
  skos:narrower wetaxtop:ReCertification, wetaxtop:Recycling, wetaxtop:Repowering, wetaxtop:Revamping;
  skos:prefLabel "End-of-Life Extension"@en .

wetaxtop:ReCertification a skos:Concept;
  dct:contributor <https://orcid.org/0000-0002-9381-9693>;
  dct:creator <http://orcid.org/0000-0003-4124-9040>;
  skos:broader wetaxtop:EndofLifeExtension;
  skos:inScheme <http://data.windenergy.dtu.dk/controlled-terminology/taxonomy-topics/>;
  skos:prefLabel "Re-Certification"@en .

wetaxtop:Recycling a skos:Concept;
  dct:contributor <https://orcid.org/0000-0002-9381-9693>;
  dct:creator <http://orcid.org/0000-0003-4124-9040>;
  skos:broader wetaxtop:EndofLifeExtension;
  skos:inScheme <http://data.windenergy.dtu.dk/controlled-terminology/taxonomy-topics/>;
  skos:prefLabel "Recycling"@en .

wetaxtop:Repowering a skos:Concept;
  dct:contributor <https://orcid.org/0000-0002-9381-9693>;
  dct:creator <http://orcid.org/0000-0003-4124-9040>;
  skos:broader wetaxtop:EndofLifeExtension;
  skos:definition "Wind turbines are dismantled and new wind turbines are installed in a brownfield and/or greenfield site."@en;
  skos:inScheme <http://data.windenergy.dtu.dk/controlled-terminology/taxonomy-topics/>;
  skos:prefLabel "Repowering"@en .

wetaxtop:Revamping a skos:Concept;
  dct:contributor <https://orcid.org/0000-0002-9381-9693>;
  dct:creator <http://orcid.org/0000-0003-4124-9040>;
  skos:altLabel "Enhancement"@en, "Lifetime Extension"@en, "Reactivation"@en, "Refurbishment"@en;
  skos:broader wetaxtop:EndofLifeExtension;
  skos:definition "An act of upgrading certain components of a wind turbine to extend the overall life time of the turbine (e.g. generator). The overall external layout of the farm remains unchanged (e.g. hub height, siting, size). Revamping differs from a normal operation and maintenance activities. New technology is installed or components are replaced instead of the initial equipment of the turbine."@en;
  skos:inScheme <http://data.windenergy.dtu.dk/controlled-terminology/taxonomy-topics/>;
  skos:prefLabel "Revamping"@en .

wetaxtop:Forecasting a skos:Concept;
  dct:contributor <https://orcid.org/0000-0002-9381-9693>;
  dct:creator <http://orcid.org/0000-0003-4124-9040>;
  skos:broader wetaxtop:OperationMaintenance;
  skos:definition "An estimate of the expected parameter from a system at a given future date."@en;
  skos:inScheme <http://data.windenergy.dtu.dk/controlled-terminology/taxonomy-topics/>;
  skos:prefLabel "Forecasting"@en .

wetaxtop:HealthSafety a skos:Concept;
  dct:contributor <https://orcid.org/0000-0002-9381-9693>;
  dct:creator <http://orcid.org/0000-0003-4124-9040>;
  skos:broader wetaxtop:OperationMaintenance;
  skos:inScheme <http://data.windenergy.dtu.dk/controlled-terminology/taxonomy-topics/>;
  skos:prefLabel "Health & Safety"@en .

wetaxtop:Installation a skos:Concept;
  dct:contributor <https://orcid.org/0000-0002-9381-9693>;
  dct:creator <http://orcid.org/0000-0003-4124-9040>;
  skos:broader wetaxtop:OperationMaintenance;
  skos:definition "An apparatus or a set of devices and/or apparatuses associated in a given location to fulfil specified purposes, including all means for their satisfactory operation"@en;
  skos:inScheme <http://data.windenergy.dtu.dk/controlled-terminology/taxonomy-topics/>;
  skos:prefLabel "Installation"@en .

wetaxtop:MaintenanceScheduling a skos:Concept;
  wetaxtop:IEVref "192-06"@en;
  dct:contributor <https://orcid.org/0000-0002-9381-9693>;
  dct:creator <http://orcid.org/0000-0003-4124-9040>;
  skos:broader wetaxtop:OperationMaintenance;
  skos:definition "A maintenance carried out in accordance with a specified schedule, which can identify the need for some corrective maintenance action."@en;
  skos:inScheme <http://data.windenergy.dtu.dk/controlled-terminology/taxonomy-topics/>;
  skos:prefLabel "Maintenance Scheduling"@en .

wetaxtop:Siting a skos:Concept;
  dct:contributor <https://orcid.org/0000-0002-9381-9693>;
  dct:creator <http://orcid.org/0000-0003-4124-9040>;
  skos:definition "A process of evaluating a number of factor before deciding to pursue development of a new wind farm project. These factors include: wind resource and compatibility of land/area, environmental impacts and community input (i.e., social acceptance)"@en;
  skos:inScheme <http://data.windenergy.dtu.dk/controlled-terminology/taxonomy-topics/>;
  skos:narrower wetaxtop:DesignConditions, wetaxtop:Infrastructures, wetaxtop:LongTermExtrapolation,
    wetaxtop:ResourceAssessment, wetaxtop:SpatialPlanning, wetaxtop:WindAtlas, wetaxtop:WindMapping;
  skos:prefLabel "Siting"@en;
  skos:topConceptOf <http://data.windenergy.dtu.dk/controlled-terminology/taxonomy-topics/> .

wetaxtop:DesignConditions a skos:Concept;
  wetaxtop:IEVref "415-02"@en;
  dct:contributor <https://orcid.org/0000-0002-9381-9693>;
  dct:creator <http://orcid.org/0000-0003-4124-9040>;
  skos:altLabel "Design Situation"@en;
  skos:broader wetaxtop:Siting;
  skos:definition "A possible mode of wind turbine operation, e.g. power production, parking etc."@en;
  skos:inScheme <http://data.windenergy.dtu.dk/controlled-terminology/taxonomy-topics/>;
  skos:narrower wetaxtop:Turbulence;
  skos:prefLabel "Design Conditions"@en .

wetaxtop:Turbulence a skos:Concept;
  wetaxtop:IEVref "705-04"@en;
  dct:contributor <https://orcid.org/0000-0002-9381-9693>;
  dct:creator <http://orcid.org/0000-0003-4124-9041>;
  skos:broader wetaxtop:DesignConditions;
  skos:definition "Random variations in velocity within a liquid or gaseous medium which may induce heterogeneous values of certain characteristics of the medium, such as refractive index."@en;
  skos:inScheme <http://data.windenergy.dtu.dk/controlled-terminology/taxonomy-topics/>;
  skos:prefLabel "Turbulence"@en .

wetaxtop:Infrastructures a skos:Concept;
  dct:contributor <https://orcid.org/0000-0002-9381-9693>;
  dct:creator <http://orcid.org/0000-0003-4124-9042>;
  skos:broader wetaxtop:Siting;
  skos:inScheme <http://data.windenergy.dtu.dk/controlled-terminology/taxonomy-topics/>;
  skos:prefLabel "Infrastructures"@en .

wetaxtop:LongTermExtrapolation a skos:Concept;
  dct:contributor <https://orcid.org/0000-0002-9381-9693>;
  dct:creator <http://orcid.org/0000-0003-4124-9043>;
  skos:broader wetaxtop:Siting;
  skos:definition "Long-term extrapolation involves making statistical forecasts by using historical trends that are projected for a specified period of time into the future.This type of extrapolation is only used for time-series forecasts."@en;
  skos:inScheme <http://data.windenergy.dtu.dk/controlled-terminology/taxonomy-topics/>;
  skos:prefLabel "Long-Term Extrapolation"@en .

wetaxtop:ResourceAssessment a skos:Concept;
  wetaxtop:IEVref "351-42"@en;
  dct:contributor <https://orcid.org/0000-0002-9381-9693>;
  dct:creator <http://orcid.org/0000-0003-4124-9044>;
  skos:broader wetaxtop:Siting;
  skos:definition "An estimate of the total energy production of a wind turbine generator system during a one-year period by applying the power curve to different reference wind speed frequency distributions at hub height, assuming 100% availability."@en;
  skos:inScheme <http://data.windenergy.dtu.dk/controlled-terminology/taxonomy-topics/>;
  skos:prefLabel "Resource Assessment"@en .

wetaxtop:SpatialPlanning a skos:Concept;
  dct:contributor <https://orcid.org/0000-0002-9381-9693>;
  dct:creator <http://orcid.org/0000-0003-4124-9045>;
  skos:broader wetaxtop:Siting;
  skos:inScheme <http://data.windenergy.dtu.dk/controlled-terminology/taxonomy-topics/>;
  skos:narrower wetaxtop:EnviromentalImpact, wetaxtop:LegalAspects;
  skos:prefLabel "Spatial Planning"@en .

wetaxtop:EnviromentalImpact a skos:Concept;
  wetaxtop:IEVref "904-01"@en;
  dct:contributor <https://orcid.org/0000-0002-9381-9693>;
  dct:creator <http://orcid.org/0000-0003-4124-9046>;
  skos:broader wetaxtop:SpatialPlanning;
  skos:definition "A change to the environment, whether adverse or beneficial, wholly or partly resulting from environmental aspects."@en;
  skos:editorialNote "SOURCE: IEC Guide 109:2012, 3.5, modified – The expression \"an organization's\" has been omitted."@en;
  skos:inScheme <http://data.windenergy.dtu.dk/controlled-terminology/taxonomy-topics/>;
  skos:narrower wetaxtop:NatureImpacts, wetaxtop:NoisePerception, wetaxtop:SocialAcceptance;
  skos:prefLabel "Enviromental Impact"@en .

wetaxtop:NatureImpacts a skos:Concept;
  dct:contributor <https://orcid.org/0000-0002-9381-9693>;
  dct:creator <http://orcid.org/0000-0003-4124-9047>;
  skos:broader wetaxtop:EnviromentalImpact;
  skos:inScheme <http://data.windenergy.dtu.dk/controlled-terminology/taxonomy-topics/>;
  skos:prefLabel "Nature Impacts"@en .

wetaxtop:NoisePerception a skos:Concept;
  dct:contributor <https://orcid.org/0000-0002-9381-9693>;
  dct:creator <http://orcid.org/0000-0003-4124-9048>;
  skos:broader wetaxtop:EnviromentalImpact;
  skos:definition "Individual perception of the acoustic noise level produced by a machine under specified conditions of operation and measurement."@en;
  skos:inScheme <http://data.windenergy.dtu.dk/controlled-terminology/taxonomy-topics/>;
  skos:prefLabel "Noise Perception"@en .

wetaxtop:SocialAcceptance a skos:Concept;
  dct:contributor <https://orcid.org/0000-0002-9381-9693>;
  dct:creator <http://orcid.org/0000-0003-4124-9049>;
  skos:altLabel "Community Input"@en;
  skos:broader wetaxtop:EnviromentalImpact;
  skos:inScheme <http://data.windenergy.dtu.dk/controlled-terminology/taxonomy-topics/>;
  skos:prefLabel "Social Acceptance"@en .

wetaxtop:LegalAspects a skos:Concept;
  dct:contributor <https://orcid.org/0000-0002-9381-9693>;
  dct:creator <http://orcid.org/0000-0003-4124-9050>;
  skos:broader wetaxtop:SpatialPlanning;
  skos:inScheme <http://data.windenergy.dtu.dk/controlled-terminology/taxonomy-topics/>;
  skos:prefLabel "Legal Aspects"@en .

wetaxtop:WindAtlas a skos:Concept;
  dct:contributor <https://orcid.org/0000-0002-9381-9693>;
  dct:creator <http://orcid.org/0000-0003-4124-9051>;
  skos:broader wetaxtop:Siting;
  skos:definition "A wind atlas is a systematic and comprehensive collection of generalized wind climates derived by the wind atlas methodology."@en;
  skos:inScheme <http://data.windenergy.dtu.dk/controlled-terminology/taxonomy-topics/>;
  skos:prefLabel "Wind Atlas"@en .

wetaxtop:WindMapping a skos:Concept;
  dct:contributor <https://orcid.org/0000-0002-9381-9693>;
  dct:creator <http://orcid.org/0000-0003-4124-9052>;
  skos:broader wetaxtop:Siting;
  skos:definition "A process of visualizing spatial variation of wind speed over geographic areas to help choosing prospective development areas for wind turbines installation."@en;
  skos:inScheme <http://data.windenergy.dtu.dk/controlled-terminology/taxonomy-topics/>;
  skos:prefLabel "Wind Mapping"@en .

wetaxtop:WindPowerPlant a skos:Concept;
  dct:contributor <https://orcid.org/0000-0002-9381-9693>;
  dct:creator <http://orcid.org/0000-0003-4124-9040>;
  skos:definition "A power station comprising a group or groups of wind turbines."@en;
  skos:inScheme <http://data.windenergy.dtu.dk/controlled-terminology/taxonomy-topics/>;
  skos:narrower wetaxtop:AncillaryServices, wetaxtop:GridConnection, wetaxtop:Loads,
    wetaxtop:Performance, wetaxtop:WindFarm;
  skos:prefLabel "Wind Power Plant"@en;
  skos:topConceptOf <http://data.windenergy.dtu.dk/controlled-terminology/taxonomy-topics/> .

wetaxtop:AncillaryServices a skos:Concept;
  dct:contributor <https://orcid.org/0000-0002-9381-9693>;
  dct:creator <http://orcid.org/0000-0003-4124-9049>;
  skos:broader wetaxtop:WindPowerPlant;
  skos:definition "Services necessary for the operation of an electric power system provided by the system operator and/or by power system users."@en;
  skos:inScheme <http://data.windenergy.dtu.dk/controlled-terminology/taxonomy-topics/>;
  skos:note "System ancillary services may include the participation in frequency regulation, reactive power regulation, active power reservation, etc."@en;
  skos:prefLabel "Ancillary Services"@en .

wetaxtop:GridConnection a skos:Concept;
  wetaxtop:IEVref "692-01-03"@en;
  dct:contributor <https://orcid.org/0000-0002-9381-9693>;
  dct:creator <http://orcid.org/0000-0003-4124-9050>;
  skos:broader wetaxtop:WindPowerPlant;
  skos:definition "A connection to an electric power network."@en;
  skos:inScheme <http://data.windenergy.dtu.dk/controlled-terminology/taxonomy-topics/>;
  skos:narrower wetaxtop:ArrayCables, wetaxtop:Substation, wetaxtop:TransmissionSystem;
  skos:prefLabel "Grid Connection"@en .

wetaxtop:ArrayCables a skos:Concept;
  dct:contributor <https://orcid.org/0000-0002-9381-9693>;
  dct:creator <http://orcid.org/0000-0003-4124-9051>;
  skos:broader wetaxtop:GridConnection;
  skos:inScheme <http://data.windenergy.dtu.dk/controlled-terminology/taxonomy-topics/>;
  skos:prefLabel "Array Cables"@en .

wetaxtop:Substation a skos:Concept;
  dct:contributor <https://orcid.org/0000-0002-9381-9693>;
  dct:creator <http://orcid.org/0000-0003-4124-9052>;
  skos:broader wetaxtop:GridConnection;
  skos:definition "A part of a power system, concentrated in a given place, including mainly the terminations of transmission or distribution lines switchgear and housing and which may also include transformers. It generally includes facilities necessary for system security and control (e.g. the protective devices)."@en;
  skos:inScheme <http://data.windenergy.dtu.dk/controlled-terminology/taxonomy-topics/>;
  skos:note "According to the nature of the system within which the substation is included, a prefix may qualify it."@en;
  skos:prefLabel "Substation"@en .

wetaxtop:TransmissionSystem a skos:Concept;
  wetaxtop:IEVref "704"@en;
  dct:contributor <https://orcid.org/0000-0002-9381-9693>;
  dct:creator <http://orcid.org/0000-0003-4124-9053>;
  skos:broader wetaxtop:GridConnection;
  skos:definition "Whole of the means of transmission, comprising the transmission medium, terminal equipment, any necessary intermediate equipment and any equipment provided for such ancillary purposes as power feeding, supervision and testing."@en;
  skos:inScheme <http://data.windenergy.dtu.dk/controlled-terminology/taxonomy-topics/>;
  skos:note "A transmission system is in accordance with a set of principles that is also called “transmission system” (see IEV 704-04-10)."@en;
  skos:prefLabel "Transmission System"@en .

wetaxtop:Loads a skos:Concept;
  wetaxtop:IEVref "415-02"@en;
  dct:contributor <https://orcid.org/0000-0002-9381-9693>;
  dct:creator <http://orcid.org/0000-0003-4124-9054>;
  skos:altLabel "Load Cases"@en;
  skos:broader wetaxtop:WindPowerPlant;
  skos:definition "A combination of design situations and external conditions which result in a structural loading."@en;
  skos:inScheme <http://data.windenergy.dtu.dk/controlled-terminology/taxonomy-topics/>;
  skos:prefLabel "Loads"@en .

wetaxtop:Performance a skos:Concept;
  dct:contributor <https://orcid.org/0000-0002-9381-9693>;
  dct:creator <http://orcid.org/0000-0003-4124-9055>;
  skos:broader wetaxtop:WindPowerPlant;
  skos:inScheme <http://data.windenergy.dtu.dk/controlled-terminology/taxonomy-topics/>;
  skos:prefLabel "Performance"@en .

wetaxtop:WindFarm a skos:Concept;
  wetaxtop:IEVref "415-01"@en;
  dct:contributor <https://orcid.org/0000-0002-9381-9693>;
  dct:creator <http://orcid.org/0000-0003-4124-9056>;
  skos:broader wetaxtop:WindPowerPlant;
  skos:definition "A group of wind turbine generator jointly operated."@en;
  skos:inScheme <http://data.windenergy.dtu.dk/controlled-terminology/taxonomy-topics/>;
  skos:narrower wetaxtop:Wakes, wetaxtop:WindFarmControl;
  skos:prefLabel "Wind Farm"@en .

wetaxtop:Wakes a skos:Concept;
  dct:contributor <https://orcid.org/0000-0002-9381-9693>;
  dct:creator <http://orcid.org/0000-0003-4124-9057>;
  skos:broader wetaxtop:WindFarm;
  skos:definition "A region behind the wind turbine with reduced wind speed and increased turbulence due to the extraction of energy from the wind when the flow pass through the rotor."@en;
  skos:inScheme <http://data.windenergy.dtu.dk/controlled-terminology/taxonomy-topics/>;
  skos:prefLabel "Wakes"@en .

wetaxtop:WindFarmControl a skos:Concept;
  dct:contributor <https://orcid.org/0000-0002-9381-9693>;
  dct:creator <http://orcid.org/0000-0003-4124-9058>;
  skos:broader wetaxtop:WindFarm;
  skos:definition "A sub‑system that receives information about the condition of the wind farm and/or its environment and adjusts the turbines in order to operate them within their operating limits."@en;
  skos:inScheme <http://data.windenergy.dtu.dk/controlled-terminology/taxonomy-topics/>;
  skos:prefLabel "Wind Farm Control"@en .

wetaxtop:WindTurbine a skos:Concept;
  dct:contributor <https://orcid.org/0000-0002-9381-9693>;
  dct:creator <http://orcid.org/0000-0003-4124-9040>;
  skos:definition "A rotating machinery in which the kinetic wind energy is transformed into another form of energy."@en;
  skos:inScheme <http://data.windenergy.dtu.dk/controlled-terminology/taxonomy-topics/>;
  skos:narrower wetaxtop:ConceptDesign, wetaxtop:Controls, wetaxtop:Nacelle, wetaxtop:Rotor,
    wetaxtop:SupportStructure, wetaxtop:Tower;
  skos:prefLabel "Wind Turbine"@en;
  skos:topConceptOf <http://data.windenergy.dtu.dk/controlled-terminology/taxonomy-topics/> .

wetaxtop:ConceptDesign a skos:Concept;
  dct:contributor <https://orcid.org/0000-0002-9381-9693>;
  dct:creator <http://orcid.org/0000-0003-4124-9057>;
  skos:broader wetaxtop:WindTurbine;
  skos:definition "An activity applied in order to analyse and transform specified requirements into acceptable design solutions."@en;
  skos:editorialNote "This entry was numbered 351-21-29 in IEC 60050-351:2006."@en;
  skos:inScheme <http://data.windenergy.dtu.dk/controlled-terminology/taxonomy-topics/>;
  skos:narrower wetaxtop:Aerial, wetaxtop:HorizontalAxis, wetaxtop:MonoMultiRotor, wetaxtop:VerticalAxis;
  skos:prefLabel "Concept Design"@en .

wetaxtop:Aerial a skos:Concept;
  dct:contributor <https://orcid.org/0000-0002-9381-9693>;
  dct:creator <http://orcid.org/0000-0003-4124-9058>;
  skos:altLabel "Airborne"@en;
  skos:broader wetaxtop:ConceptDesign;
  skos:definition "An aerial wind turbine is a design concept for a wind turbine with a rotor supported in the air without a tower, thus benefiting from more mechanical and aerodynamic options, the higher velocity and persistence of wind at high altitudes."@en;
  skos:inScheme <http://data.windenergy.dtu.dk/controlled-terminology/taxonomy-topics/>;
  skos:prefLabel "Aerial"@en .

wetaxtop:HorizontalAxis a skos:Concept;
  dct:contributor <https://orcid.org/0000-0002-9381-9693>;
  dct:creator <http://orcid.org/0000-0003-4124-9059>;
  skos:broader wetaxtop:ConceptDesign;
  skos:definition "A wind turbine which rotor axis is horizontal."@en;
  skos:inScheme <http://data.windenergy.dtu.dk/controlled-terminology/taxonomy-topics/>;
  skos:prefLabel "Horizontal Axis"@en .

wetaxtop:MonoMultiRotor a skos:Concept;
  dct:contributor <https://orcid.org/0000-0002-9381-9693>;
  dct:creator <http://orcid.org/0000-0003-4124-9060>;
  skos:broader wetaxtop:ConceptDesign;
  skos:definition "A wind turbine with one or more rotors, independent on the number of blades."@en;
  skos:inScheme <http://data.windenergy.dtu.dk/controlled-terminology/taxonomy-topics/>;
  skos:prefLabel "Mono-Multi Rotor"@en .

wetaxtop:VerticalAxis a skos:Concept;
  dct:contributor <https://orcid.org/0000-0002-9381-9693>;
  dct:creator <http://orcid.org/0000-0003-4124-9061>;
  skos:broader wetaxtop:ConceptDesign;
  skos:definition "A wind turbine which rotor axis is vertical."@en;
  skos:inScheme <http://data.windenergy.dtu.dk/controlled-terminology/taxonomy-topics/>;
  skos:prefLabel "Vertical Axis"@en .

wetaxtop:Controls a skos:Concept;
  dct:contributor <https://orcid.org/0000-0002-9381-9693>;
  dct:creator <http://orcid.org/0000-0003-4124-9062>;
  skos:broader wetaxtop:WindTurbine;
  skos:definition "A purposeful action on or in a process to meet specified objectives."@en;
  skos:inScheme <http://data.windenergy.dtu.dk/controlled-terminology/taxonomy-topics/>;
  skos:narrower wetaxtop:BlackBox;
  skos:prefLabel "Controls"@en .

wetaxtop:BlackBox a skos:Concept;
  dct:contributor <https://orcid.org/0000-0002-9381-9693>;
  dct:creator <http://orcid.org/0000-0003-4124-9063>;
  skos:broader wetaxtop:Controls;
  skos:inScheme <http://data.windenergy.dtu.dk/controlled-terminology/taxonomy-topics/>;
  skos:prefLabel "Black-Box"@en .

wetaxtop:Nacelle a skos:Concept;
  dct:contributor <https://orcid.org/0000-0002-9381-9693>;
  dct:creator <http://orcid.org/0000-0003-4124-9064>;
  skos:broader wetaxtop:WindTurbine;
  skos:definition "A housing which contains the drive‑train and other elements on top of a horizontal axis wind turbine tower."@en;
  skos:inScheme <http://data.windenergy.dtu.dk/controlled-terminology/taxonomy-topics/>;
  skos:narrower wetaxtop:Cooling, wetaxtop:Gearbox, wetaxtop:Generator, wetaxtop:MainShaft,
    wetaxtop:PowerElectronics, wetaxtop:TurbineControl;
  skos:prefLabel "Nacelle"@en .

wetaxtop:Cooling a skos:Concept;
  wetaxtop:IEVref "411-44"@en;
  dct:contributor <https://orcid.org/0000-0002-9381-9693>;
  dct:creator <http://orcid.org/0000-0003-4124-9065>;
  skos:broader wetaxtop:Nacelle;
  skos:definition "A procedure by means of which heat resulting from losses occurring in a machine is given up to a primary coolant which may be continuously replaced or may itself be cooled by a secondary coolant in a heat exchanger."@en;
  skos:inScheme <http://data.windenergy.dtu.dk/controlled-terminology/taxonomy-topics/>;
  skos:prefLabel "Cooling"@en .

wetaxtop:Gearbox a skos:Concept;
  dct:contributor <https://orcid.org/0000-0002-9381-9693>;
  dct:creator <http://orcid.org/0000-0003-4124-9066>;
  skos:broader wetaxtop:Nacelle;
  skos:definition "A protective casing providing a reservoir of oil or grease for the gearing."@en;
  skos:inScheme <http://data.windenergy.dtu.dk/controlled-terminology/taxonomy-topics/>;
  skos:prefLabel "Gearbox"@en .

wetaxtop:Generator a skos:Concept;
  dct:contributor <https://orcid.org/0000-0002-9381-9693>;
  dct:creator <http://orcid.org/0000-0003-4124-9067>;
  skos:broader wetaxtop:Nacelle;
  skos:definition "A machine which converts mechanical energy into electrical energy."@en;
  skos:inScheme <http://data.windenergy.dtu.dk/controlled-terminology/taxonomy-topics/>;
  skos:prefLabel "Generator"@en .

wetaxtop:MainShaft a skos:Concept;
  dct:contributor <https://orcid.org/0000-0002-9381-9693>;
  dct:creator <http://orcid.org/0000-0003-4124-9068>;
  skos:broader wetaxtop:Nacelle;
  skos:inScheme <http://data.windenergy.dtu.dk/controlled-terminology/taxonomy-topics/>;
  skos:prefLabel "Main Shaft"@en .

wetaxtop:PowerElectronics a skos:Concept;
  dct:contributor <https://orcid.org/0000-0002-9381-9693>;
  dct:creator <http://orcid.org/0000-0003-4124-9069>;
  skos:broader wetaxtop:Nacelle;
  skos:definition "A field of electronics which deals with the conversion or switching of electric power with or without control of that power."@en;
  skos:inScheme <http://data.windenergy.dtu.dk/controlled-terminology/taxonomy-topics/>;
  skos:prefLabel "Power Electronics"@en .

wetaxtop:TurbineControl a skos:Concept;
  dct:contributor <https://orcid.org/0000-0002-9381-9693>;
  dct:creator <http://orcid.org/0000-0003-4124-9070>;
  skos:broader wetaxtop:Nacelle;
  skos:definition "A wind turbine sub‑system that receives information about the condition of the wind turbine and/or its environment and adjusts the turbine in order to operate it within its operating limits."@en;
  skos:inScheme <http://data.windenergy.dtu.dk/controlled-terminology/taxonomy-topics/>;
  skos:prefLabel "Turbine Control"@en .

wetaxtop:Rotor a skos:Concept;
  dct:contributor <https://orcid.org/0000-0002-9381-9693>;
  dct:creator <http://orcid.org/0000-0003-4124-9071>;
  skos:broader wetaxtop:WindTurbine;
  skos:definition "One of the main part of a wind turbine"@en;
  skos:inScheme <http://data.windenergy.dtu.dk/controlled-terminology/taxonomy-topics/>;
  skos:narrower wetaxtop:Blades, wetaxtop:Hub;
  skos:prefLabel "Rotor"@en .

wetaxtop:Blades a skos:Concept;
  dct:contributor <https://orcid.org/0000-0002-9381-9693>;
  dct:creator <http://orcid.org/0000-0003-4124-9072>;
  skos:broader wetaxtop:Rotor;
  skos:definition "Components of a wind turbine that harness wind energy and drive the rotor of a wind turbine."@en;
  skos:inScheme <http://data.windenergy.dtu.dk/controlled-terminology/taxonomy-topics/>;
  skos:prefLabel "Blades"@en .

wetaxtop:Hub a skos:Concept;
  dct:contributor <https://orcid.org/0000-0002-9381-9693>;
  dct:creator <http://orcid.org/0000-0003-4124-9073>;
  skos:broader wetaxtop:Rotor;
  skos:definition "A fixture for attaching the blades or blade assembly to the rotor shaft."@en;
  skos:inScheme <http://data.windenergy.dtu.dk/controlled-terminology/taxonomy-topics/>;
  skos:prefLabel "Hub"@en .

wetaxtop:SupportStructure a skos:Concept;
  dct:contributor <https://orcid.org/0000-0002-9381-9693>;
  dct:creator <http://orcid.org/0000-0003-4124-9074>;
  skos:broader wetaxtop:WindTurbine;
  skos:definition "A part of a wind turbine comprising the tower and foundation."@en;
  skos:inScheme <http://data.windenergy.dtu.dk/controlled-terminology/taxonomy-topics/>;
  skos:narrower wetaxtop:Floating, wetaxtop:Foundation, wetaxtop:MooringLines, wetaxtop:Substructure;
  skos:prefLabel "Support Structure"@en .

wetaxtop:Floating a skos:Concept;
  dct:contributor <https://orcid.org/0000-0002-9381-9693>;
  dct:creator <http://orcid.org/0000-0003-4124-9075>;
  skos:broader wetaxtop:SupportStructure;
  skos:inScheme <http://data.windenergy.dtu.dk/controlled-terminology/taxonomy-topics/>;
  skos:prefLabel "Floating"@en .

wetaxtop:Foundation a skos:Concept;
  dct:contributor <https://orcid.org/0000-0002-9381-9693>;
  dct:creator <http://orcid.org/0000-0003-4124-9076>;
  skos:broader wetaxtop:SupportStructure;
  skos:definition "A structure set in the ground, to which the base of a support is attached to provide the necessary anchorage to withstand all applied loads."@en;
  skos:inScheme <http://data.windenergy.dtu.dk/controlled-terminology/taxonomy-topics/>;
  skos:prefLabel "Foundation"@en .

wetaxtop:MooringLines a skos:Concept;
  dct:contributor <https://orcid.org/0000-0002-9381-9693>;
  dct:creator <http://orcid.org/0000-0003-4124-9077>;
  skos:broader wetaxtop:SupportStructure;
  skos:inScheme <http://data.windenergy.dtu.dk/controlled-terminology/taxonomy-topics/>;
  skos:prefLabel "Mooring Lines"@en .

wetaxtop:Substructure a skos:Concept;
  dct:contributor <https://orcid.org/0000-0002-9381-9693>;
  dct:creator <http://orcid.org/0000-0003-4124-9078>;
  skos:broader wetaxtop:SupportStructure;
  skos:inScheme <http://data.windenergy.dtu.dk/controlled-terminology/taxonomy-topics/>;
  skos:prefLabel "Substructure"@en .

wetaxtop:Tower a skos:Concept;
  dct:contributor <https://orcid.org/0000-0002-9381-9693>;
  dct:creator <http://orcid.org/0000-0003-4124-9079>;
  skos:broader wetaxtop:WindTurbine;
  skos:definition "A support which may be made of such material as steel, wood, concrete, and comprising a body which is normally four-sided, and cross-arms."@en;
  skos:inScheme <http://data.windenergy.dtu.dk/controlled-terminology/taxonomy-topics/>;
  skos:narrower wetaxtop:Lattice, wetaxtop:Tubular;
  skos:prefLabel "Tower"@en .

wetaxtop:Tubular a skos:Concept;
  dct:contributor <https://orcid.org/0000-0002-9381-9693>;
  dct:creator <http://orcid.org/0000-0003-4124-9080>;
  skos:broader wetaxtop:Tower;
  skos:definition "A structure of a tower having the form or shape of a tube slightly conical (i.e. with their diameter increasing towards the base) in order to increase their strength and to save materials at the same time."@en;
  skos:inScheme <http://data.windenergy.dtu.dk/controlled-terminology/taxonomy-topics/>;
  skos:prefLabel "Tubular"@en .

wetaxtop:Lattice a skos:Concept;
  dct:contributor <https://orcid.org/0000-0002-9381-9693>;
  dct:creator <http://orcid.org/0000-0003-4124-9081>;
  skos:broader wetaxtop:Tower;
  skos:definition "A structure consisting of strips of wood or metal crossed and fastened together with square-shaped spaces left between, used as a support for climbing plants."@en;
  skos:inScheme <http://data.windenergy.dtu.dk/controlled-terminology/taxonomy-topics/>;
  skos:prefLabel "Lattice"@en .
